user 5, session 35, part 7

diffs-annotated/5/user-5-session-35.v
@@ -189,10 +189,33 @@ Fixpoint free_vars (t : Term) : list Identifier :=
   | Choose x P =>
       filter (fun y => if id_eq_dec x y then false else true) (free_vars P)
   end.
+Axiom (fresh_var : list Identifier -> Identifier).
 Axiom
   (fresh_var_unique : forall exclude, ~ List.In (fresh_var exclude) exclude).
+Definition Divide (t1 : Term) (t2 : Term) :=
+  let x := fresh_var (free_vars t1 ++ free_vars t2) in
+  Choose x (And (In (Var x) Ints) (Eq t1 (Times (Var x) t2))).
+Lemma extendEnv_eq :
+  forall Value env x (val : Value), (extendEnv env x val) x = val.
+Proof.
+(intros).
+(unfold extendEnv).
+(destruct (id_eq_dec x x); congruence).
+Qed.
+Lemma divide_test :
+  forall L env, L.(eval) env (Divide (Int 6) (Int 2)) = L.(eval) env (Int 3).
+Proof.
+(intros).
+(unfold Divide).
+(match goal with
+ | |- context [ Choose ?x _ ] => generalize x
+ end).
+intro x.
 (assert
   (forall res,
    eval L env
      (Choose x (And (In (Var x) Ints) (Eq (Int 6) (Times (Var x) (Int 2))))) =
    res -> exists i, res = eval L env (Int i))).
+{
+(intros).
+apply -> evalInInts.
